\documentclass[11pt]{article}
\usepackage[margin=1.0in]{geometry}
\usepackage{amsmath}
\usepackage{url,  multirow}
\usepackage{booktabs}
\usepackage{longtable}

\title{Equations}
\author{Me\\Here}
\date{\today}


\begin{document}

\maketitle
\tableofcontents

\section*{Appendix 1}

\begin{longtable}{lp{12cm}} 
%\begin{tabular}{lp{10cm}}
\toprule

% Population dynamics
\textbf{Population dynamics} &
 \begin{equation} N_{a+1, y+1} = N_{a,y} e^{-Z_{a,y}} \end{equation} \\
%
 &
 \begin{equation} N_{p,y} = N_{p-1, y-1} e^{-Z_{p-1, y-1}} + N_{p,y} e ^{-Z_{p, y-1}} \end{equation} \\
%
 &  \begin{equation} N_{r,y} = f(B_{y-r}) \end{equation} \\
\midrule

% Mortality rates
\textbf{Mortality rates} & \begin{equation} Z_{a,y} = F_{a,y} + D_{a,y} + M_{a,y} \end{equation} \\
%
 & \begin{subequations} 
\begin{equation} F_{a,y} = \sum_{i=1}^f P_{i,a,y} S_{i,a,y} E_{i,y} \end{equation}
\begin{equation} D_{a,y} = \sum_{i=1}^f \left(1- P_{i,a,y}\right) S_{i,a,y} E_{i,y} \end{equation}
\end{subequations}\\
\midrule

% Catch equation
\textbf{Catch equation} & \begin{equation} C_{f,a,y} = N_{a,y} \frac{F_{f,a,y}}{Z_{f,a,y}} \left(1 - e^{-Z_{a,y}} \right) \end{equation} \\
\midrule

%
\multicolumn{2}{l}{\textbf{Stock recruitment relationships}} \\
\addlinespace
% BH
Beverton \& Holt & \begin{equation} N_{r,y} = \frac{B_{y-r}}{\alpha B_{y-r} + \beta} \end{equation} \\
% BB
\bottomrule

\multicolumn{2}{l}{\textbf{Growth and maturity}} \\
% BH
von Bertalanffy & \begin{equation} N_{r,y} = \frac{B_{y-r}}{\alpha B_{y-r} + \beta} \end{equation} \\
\bottomrule

\multicolumn{2}{l}{\textbf{Equilibrium Calculations}} \\
Spawner-per-recruit & 
\begin{equation} S/R=\sum\limits_{a=r}^{n-1} {e^{\sum\limits_{i=r}^{a-1} {-F_i-M_i}}} W_a Q_a + e^{\sum\limits_{i=r}^{n-1} {-F_n-M_n}} \frac{W_n Q_n}{1-e_{-F_n-M_n}} 
\end{equation} \\

Yield-per-recruit &
\begin{equation}
\begin{aligned}
Y/R=\sum\limits_{a=r}^{n-1} {e^{\sum\limits_{i=r}^{a-1} {-F_i-M_i}}} W_a\frac{F_a}{F_a+M_a}\left(1-e^{-F_i-M_i}  \right) +\\
e^{\sum\limits_{i=r}^{n-1} {-F_n-M_n}} W_n\frac{F_n}{F_n+M_n}
\end{aligned}
\end{equation} \\

~ &
\begin{equation}
R=\frac{aS}{S+b}
\end{equation} \\


\bottomrule
%\end{tabular}
\end{longtable}
\end{document}

~ & \begin{equation}
R=aS^e{-bS} \\
\end{equation} 

~ & \begin{equation}
\tau=a\frac{\left({S/R}\right)_{F=0}}{4b+a\left(S/R\right)_{F=0}} \\
\end{equation}

~ & \begin{equation}
\lambda=a\frac{\left({S/R}\right)_{F=0}}{4b+a\left({S/R}\right)_{F=0}} \\
\end{equation}

~ & \begin{equation}
\gamma=\frac{log\left[\left({S/R}\right)_{F=0}\right]}{b} \\
\end{equation}

~ & \begin{equation}
\tau=0.2e^{0.8b\lambda} \\
\end{equation}

~ & \begin{equation}
R=a-\frac{β}{S/R} \\
\end{equation}

~ & \begin{equation}
{R={\frac{alog\left(a\left(S/R\right)\right)}{β}}e^{{-a\left(S/R\right)}}} \\
\end{equation}

~ & \begin{equation}
L_a=L_{\infty}\left(1-e^K\right) \\
\end{equation}

~ & \begin{equation}
M=e^{\left[a+b.log\left(L_{\infty}\right)+clog\left({\bar{L}}\right)+dlog\left(K\right)\right]} \\
\end{equation}

~ & \begin{equation}
log(M)= e^{1.44-0.982log(maxAge)} \\
\end{equation}

~ & \begin{equation}
{a{{MAT}}=log{\frac{\left(\frac{3K+M}{M}\right)}{K}}} \\
\end{equation}

~ & \begin{equation}
m\left(a\right)={\frac{1}{1+e^{\left[-\eta{{m}}\left(a-a{{MAT}}\right)\right]}}} \\
\end{equation}

~ & \begin{equation}
f\left(x\right) = \left\{ 
\begin{array}{ll}
         exp\left[\left(-x-a_1\right)^2/\sigma_l\right], & \mbox{if $x \leq a_1$}\\
         exp\left[\left(-x-a_1\right)^2/\sigma_r\right], & \mbox{if $x > a_1$}   \\
\end{array}\right
\end{equation}
\bottomrule


% Biomass Dynamic
\multicolumn{2}{l}{\textbf{Biomass Dynamic}} \\
\addlinespace
Population Dynamics	& \begin{equation} B_{t+1} = B_t + P_t -C_t \end{equation} \\
\bottomrule

\multicolumn{2}{l}{\textbf{Biomass Dynamic Surplus Production Functions}} \\
\addlinespace
Schaefer 		& \begin{equation} N_{r,y} = \frac{B_{y-r}}{\alpha B_{y-r} + \beta} \end{equation} \\
Gompertz		& \begin{equation} N_{r,y} = \frac{B_{y-r}}{\alpha B_{y-r} + \beta} \end{equation} \\
Pella and Tomlinson	& \begin{equation} N_{r,y} = \frac{B_{y-r}}{\alpha B_{y-r} + \beta} \end{equation} \\
Theta-logistic		& \begin{equation} N_{r,y} = \frac{B_{y-r}}{\alpha B_{y-r} + \beta} \end{equation} \\
Fletcher		& \begin{equation} N_{r,y} = \frac{B_{y-r}}{\alpha B_{y-r} + \beta} \end{equation} \\
Polacheck		& \begin{equation} N_{r,y} = \frac{B_{y-r}}{\alpha B_{y-r} + \beta} \end{equation} \\
Shepherd		& \begin{equation} N_{r,y} = \frac{B_{y-r}}{\alpha B_{y-r} + \beta} \end{equation} \\
Fox			& \begin{equation} N_{r,y} = \frac{B_{y-r}}{\alpha B_{y-r} + \beta} \end{equation} \\
Gulland			& \begin{equation} N_{r,y} = \frac{B_{y-r}}{\alpha B_{y-r} + \beta} \end{equation} \\
\bottomrule

\multicolumn{2}{l}{\textbf{Biomass Dynamic MSY Reference Points}} \\
\addlinespace
Schaefer 		& \begin{equation} B_{y-r} \end{equation} \\
Gompertz		& \begin{equation} B_{y-r} \end{equation} \\
Pella and Tomlinson	& \begin{equation} B_{y-r} \end{equation} \\
Theta-logistic		& \begin{equation} B_{y-r} \end{equation} \\
Fletcher		& \begin{equation} B_{y-r} \end{equation} \\
Polacheck		& \begin{equation} B_{y-r} \end{equation} \\
Shepherd		& \begin{equation} B_{y-r} \end{equation} \\
Fox			& \begin{equation} B_{y-r} \end{equation} \\
Gulland			& \begin{equation} B_{y-r} \end{equation} \\


\multicolumn{2}{l}{\textbf{Biomass Dynamic B_{MSY} Reference Points}} \\
\addlinespace
Schaefer 		& \begin{equation} B_{y-r} \end{equation} \\
Gompertz		& \begin{equation} B_{y-r} \end{equation} \\
Pella and Tomlinson	& \begin{equation} B_{y-r} \end{equation} \\
Theta-logistic		& \begin{equation} B_{y-r} \end{equation} \\
Fletcher		& \begin{equation} B_{y-r} \end{equation} \\
Polacheck		& \begin{equation} B_{y-r} \end{equation} \\
Shepherd		& \begin{equation} B_{y-r} \end{equation} \\
Fox			& \begin{equation} B_{y-r} \end{equation} \\
Gulland			& \begin{equation} B_{y-r} \end{equation} \\
\bottomrule
\end{tabular}


\begin{eqnarray*}
  g(B) &=& rB\,(\log K\!-\!\log B)                                      \\[1em]
  ~    &=& rB\,\log K\!\left(1-\frac{\,\log B\,}{\log K}\right)         \\[1em]
\end{eqnarray*}


Pella and Tomlinson (1969)

\begin{eqnarray*}
  g(B) &=& \mathcal{H}B^m \;-\; \mathcal{K}B\\[1ex]
   ~   &=& \frac{\,rB\,}{p}\!
     \left[\,1 \;-\; \left(\frac{B}{K}\right)^{\!p}\,\right]
\end{eqnarray*}



Theta-logistic

\begin{eqnarray*}
  g(B) &=& rB\!\left[\,1\!-\!\left(\frac{B}{K}\right)^{\!\theta}\:\right]\\[1ex]
\end{eqnarray*}

Fletcher (1978)

\begin{eqnarray*}
  g(B) &=& \gamma m\frac{B}{K}\left[\,1 \;-\;
    \left(\frac{B}{K}\right)^{\!\!n-1}\,\right]\\[1ex]
\end{eqnarray*}


Polacheck et al. (1993)

\begin{eqnarray*}
  g(B) &=& \frac{r}{p}\,B\!
  \left[\,1\!-\!\left(\frac{B}{K}\right)^{\!p}\,\right]\\[1ex]
\end{eqnarray*}


\end{document}
